- 제 1법칙
	행성은 모행성을 한 초점으로 하는 타원궤도를 그리며 공전 (타원궤도 법칙)

- 제 2법칙
	면적 속도 일정의 법칙

- 제 3법칙
	조화의 법칙 ($P^{2} \propto a^{3}$)


![[스크린샷 2023-07-12 오후 7.35.52.png|400x200]]
we want to find $r(t)$ and $\theta(t)$.

by Newton law,
$$
\begin{align}
\vec{F} &= m\vec{a} \\
&= \vec{F_{r}}\hat{r} + \vec{F_\theta}\hat{\theta}
\end{align} \tag{2.1.1}$$
Then
$$
\begin{align}
F_{r}&=-\frac{GMm}{r^{2}} = ma_{r}=m(\ddot{r}-r\dot{\theta}^{2}) \\
F_{\theta}&= 0
\end{align} \tag{2.1.2}
$$
so the angular momentum conserves.
$$
\begin{align}
&L = mv_{\bot}r = mwr^2=m\left(\frac{d\theta}{dt}\right)r^{2}
\\
&\therefore \left(\frac{d\theta}{dt}\right)=\frac{L}{mr^{2}}
\end{align} \tag{2.1.3}
$$
**Substitution #1:** Eliminate the $\left(\dfrac{d\theta}{dt}\right)$ term from the equation $(2.1.2)$
Therefore
$$
\begin{align}
&-\frac{GMm}{r^{2}} = m(\ddot{r}-r\dot{\theta}^{2}) =m\left(\ddot{r}-r\left(\frac{L}{mr^{2}}\right)^{2}\right) \\
&\therefore \ddot{r}  - \frac{L^{2}}{m^{2}r^{3}} + \frac{GM}{r^{2}} = 0
\end{align} \tag{2.1.4}
$$
This equation is difficult to solve. We will therefore use the chain rule of differentiation to find an equation for $r(\theta)$ instead of $r(t)$

Thus, 
$$
\begin{align}
\frac{dr}{dt}  &= \left(\frac{dr}{d\theta}\right)  \left(\frac{d\theta}{dt}\right) = \frac{L}{mr^{2}} \left(\frac{dr}{d\theta}\right) \\
\frac{d^{2} r}{dt^{2}}&= \frac{d}{dt} \left[ \frac{L}{mr^{2}} \left(\frac{dr}{d\theta}\right) \right] = \left(\frac{d\theta}{dt}\right) \frac{d}{d\theta} \left[ \frac{L}{mr^{2}} \left(\frac{dr}{d\theta}\right) \right] \\
&=\frac{L}{mr^{2}} \frac{d}{d\theta} \left[ \frac{L}{mr^{2}} \left(\frac{dr}{d\theta}\right) \right] = \frac{L^{2}}{m^{2}r^{2}} \frac{d}{d\theta} \left[ \frac{1}{r^{2}} \left(\frac{dr}{d\theta}\right) \right] 
\end{align} \tag{2.1.5}
$$
put $(2.1.5)$ at $(2.1.4)$
$$
\begin{align}
\frac{L^{2}}{m^{2}r^{2}} \frac{d}{d\theta} \left[ \frac{1}{r^{2}} \left(\frac{dr}{d\theta}\right) \right] + \frac{GM}{r^{2}} - \frac{L^{2}}{m^{2}r^{3}} = 0 \\
\frac{d}{d\theta} \left[ \frac{1}{r^{2}} \left(\frac{dr}{d\theta}\right) \right] + \frac{GMm^{2}}{L^{2}} - \frac{1}{r} = 0 
\end{align} \tag{2.1.6}
$$
trick) $r\equiv\dfrac{1}{u}$
$$
\begin{align}
&\frac{d}{d\theta} \left[ u^{2} \frac{d}{d\theta}\left(\frac{1}{u}\right) \right] + \frac{GMm^{2}}{L^{2}} - u = 0 \\
&\Leftrightarrow \frac{d}{d\theta} \left[ u^{2} \left(-\frac{1}{u^{2}}\right) \frac{du}{d\theta} \right] + \frac{GMm^{2}}{L^{2}} - u = 0 \\
&\Leftrightarrow \boxed{ \frac{d^{2}u}{d\theta^{2}}  - \frac{GMm^{2}}{L^{2}} + u = 0} \tag{2.1.7}
\end{align} 
$$
Solving this differential equation of $u$ is very easy.
$$
u(\theta) = B \cos (\theta+\beta) + \frac{GMm^{2}}{L^{2}} \tag{2.1.8}
$$
We could set the apogee as a initial point ($\beta=0$), then
$$
\begin{align}
r(\theta) &= \frac{1}{B \cos \theta + GMm^{2}/L^{2}} \\
&= \boxed{\frac{L^{2}/GMm^{2}}{BL^{2}\cos\theta/GMm^{2}+1}}\tag{2.1.8}
\end{align}
$$
We could see that the expression of $r(\theta)$ has the shape of an ellipse. **First law proved.**

So as a last step, the constant B have to be determined. 

For arbitrary ellipse,
![[스크린샷 2023-07-12 오후 9.58.55.png|400x200]]
By cosine law and properties of an ellipse, ($r+r'=2a,\,\, a^{2}e^{2}+b^{2}=a^{2}$)
$$
\begin{align}
{r'}^{2} = r^{2}+ (2ae)^{2}-4aer \cos \theta \\
(2a-r)^{2}=r^{2}+ (2ae)^{2}-4aer \cos \theta \\
4a^{2}-4ar+r^{2}=r^{2}+ (2ae)^{2}-4aer \cos \theta \\
a^{2}-ar=a^{2}e^{2}-aer \cos \theta \\
ar(e \cos \theta - 1) = a^{2}(e^{2}-1) \\
\therefore \boxed{r = \frac{a(1-e^{2})}{1-e \cos \theta}} \tag{2.1.9}
\end{align}
$$
by using $(2.1.8)=(2.1.9)$,
$$
\begin{align}
a(1-e^{2})=\frac{L^{2}}{GMm^{2},} \\ 
B=-GMm^{2}e/L^{2}
\end{align} \tag{2.1.10}
$$

Recall) Since $L=m\left(\dfrac{d\theta}{dt}\right)r^{2}=const$ by angular momentum conservation,
$$
\frac{dA}{dt} = \frac{1}{2} r^{2}\frac{d\theta}{dt} = \frac{L}{2m} = const \tag{2.1.11}
$$
**Second law proved.**

As we know that the area of ellipse is $\pi ab$, Let $P$ is the period of the elliptical motion.
$$
\int^{P}_{0} \left(\frac{dA}{dt}\right) dt =A=\pi ab = \frac{L}{2m}\cdot P \tag{2.1.12}
$$
Therefore
$$
\begin{align}
\therefore P&=\frac{2\pi mab}{L}\\
P^{2}&=\frac{4\pi^{2}m^{2}a^{4}(1-e^{2})}{L^{2}} \\
&=\frac{4\pi^{2}a^{3}}{GM} (\mathrm{using} \,(2.1.10)) \\
\end{align}
$$
$$
\therefore \boxed{\left( \frac{P}{2\pi} \right)^{2} = \frac{a^{3}}{GM}}
$$
**Third law proved.**



